work on realizer proofs

Common/Reduction.lean
@@ -1,10 +1,19 @@
 import Common.Substitution
 
-class ReductionCompletion (T : Type u) (R : T -> T -> Prop) where
-  compl : T -> T
+class ReductionRespectsSubstitution (T : Type u) [SubstitutionType T] [SubstitutionTypeLaws T] (R : T -> T -> Prop) where
+  subst  σ : R t s -> R ([σ]t) ([σ]s)
 
-class ReductionTriangle (T : Type u) (R : T -> T -> Prop) [ReductionCompletion T R] where
-  triangle : R t s -> R s (ReductionCompletion.compl R t)
+class ReductionRespectsReducingSubstitution (T : Type u) [SubstitutionType T] [SubstitutionTypeLaws T] (R : T -> T -> Prop) where
+  refl t : R t t
+  subst σ τ :
+    (∀ n t, σ n = .su t -> ∃ t', τ n = .su t' ∧ R t t') ->
+    (∀ n k, σ n = .re k -> τ n = .re k) ->
+    R t s ->
+    R ([σ]t) ([τ]s)
+
+class ReductionTriangle (T : Type u) (R : T -> T -> Prop) where
+  compl : T -> T
+  triangle : R t s -> R s (compl t)
 
 variable {T : Type u} {R : T -> T -> Prop}
 
@@ -27,108 +36,22 @@ def Conv (R : T -> T -> Prop) (x y : T) : Prop :=
   ∃ z, Star R x z ∧ Star R y z
 
 namespace Star
-  theorem trans : @Star T R x y -> @Star T R y z -> @Star T R x z := by
+  theorem trans : Star R x y -> Star R y z -> Star R x z := by
   intro r1 r2; induction r2 generalizing x
   case _ => apply r1
   case _ a b _ r2 ih => apply Star.step (ih r1) r2
 
   theorem promote (Rprm : ∀ {x y}, R1 x y -> R2 x y) :
-    @Star T R1 x y -> @Star T R2 x y
-  := by
-  intro r; induction r
-  case _ => constructor
-  case _ _ r ih => constructor; apply ih; apply Rprm r
-end Star
-
-namespace Plus
-  theorem destruct : @Plus T R x z -> ∃ y, R x y ∧ @Star T R y z := by
-  intro r; induction r
-  case _ b r =>
-    exists b; apply And.intro r Star.refl
-  case _ r1 r2 ih =>
-    cases ih; case _ u ih =>
-      exists u; apply And.intro ih.1
-      apply Star.step ih.2 r2
-
-  theorem stepr : R x y -> @Plus T R y z -> @Plus T R x z := by
-  intro r1 r2
-  induction r2 generalizing x
-  case _ r2 => apply Plus.step (Plus.start r1) r2
-  case _ r3 r4 ih => apply Plus.step (ih r1) r4
-
-  theorem stepr_from_star : R x y -> @Star T R y z -> @Plus T R x z := by
-  intro r1 r2
-  induction r2 generalizing x
-  case _ => apply Plus.start; apply r1
-  case _ r3 r4 ih => apply Plus.step (ih r1) r4
-end Plus
-
-namespace StarB
-  @[simp]
-  def star (f : T -> T) : Nat -> T -> T
-  | 0, t => t
-  | n + 1, t => star f n (f t)
-
-  theorem weaken k : @StarB T R g x y -> @StarB T R (g + k) x y := by
-  intro r; induction r generalizing k
-  case _ => constructor
-  case _ n _ _ _ _ r2 ih =>
-    have lem : n + 1 + k = n + k + 1 := by omega
-    rw [lem]; apply StarB.step (ih k) r2
-
-  theorem trans : @StarB T R g1 x y -> @StarB T R g2 y z -> @StarB T R (g1 + g2) x z := by
-  intro r1 r2; induction r2 generalizing g1 x
-  case _ n t => apply weaken n r1
-  case _ n a b c _ r2 ih => apply StarB.step (ih r1) r2
-
-  theorem promote (Rprm : ∀ {x y}, R1 x y -> R2 x y) :
-    @StarB T R1 n x y -> @StarB T R2 n x y
+    Star R1 x y -> Star R2 x y
   := by
   intro r; induction r
   case _ => constructor
   case _ _ r ih => constructor; apply ih; apply Rprm r
 
-  theorem star_sound n t : (∀ t, R t (f t)) -> @StarB T R n t (star f n t) := by
-  intro h
-  have lem : ∀ {t n}, R (star f n t) (star f n (f t)) := by
-    intro t n; induction n generalizing t; simp; apply h _
-    case _ n ih => simp; apply ih
-  induction n
-  case _ => simp; constructor
-  case _ n ih =>
-    constructor; apply ih; simp; apply lem
-end StarB
-
-namespace ConvB
-  @[simp]
-  def convb [BEq T] (f : T -> T) (g1 g2 : Nat) (a b : T) : Bool :=
-    StarB.star f g1 a == StarB.star f g2 b
-
-  theorem weaken k1 k2 : @ConvB T R g1 g2 x y -> @ConvB T R (g1 + k1) (g2 + k2) x y := by
-  intro h; cases h; case _ w h =>
-    exists w; apply And.intro
-    apply StarB.weaken k1 h.1; apply StarB.weaken k2 h.2
-
-  theorem promote (Rprm : ∀ {x y}, R1 x y -> R2 x y) :
-    @ConvB T R1 g1 g2 x y -> @ConvB T R2 g1 g2 x y
-  := by
-  intro h; cases h; case _ w h =>
-    exists w; apply And.intro
-    apply StarB.promote Rprm h.1; apply StarB.promote Rprm h.2
-
-  theorem conv_sound [BEq T] [LawfulBEq T] : (∀ t, R t (f t)) -> convb f g1 g2 a b -> @ConvB T R g1 g2 a b := by
-  intro h1 h2; simp at h2
-  have lem1 := StarB.star_sound g1 a h1
-  have lem2 := StarB.star_sound g2 b h1
-  exists (StarB.star f g1 a); apply And.intro
-  apply lem1; rw [h2]; apply lem2
-end ConvB
-
-namespace Star
   theorem congr3_1 t2 t3 (f : T -> T -> T -> T) :
-    (∀ {t1 t2 t3 t1'}, R t1 t1' -> R (f t1 t2 t3) (f t1' t2 t3)) ->
-    @Star T R t1 t1' ->
-    @Star T R (f t1 t2 t3) (f t1' t2 t3)
+  (∀ {t1 t2 t3 t1'}, R t1 t1' -> R (f t1 t2 t3) (f t1' t2 t3)) ->
+  Star R t1 t1' ->
+  Star R (f t1 t2 t3) (f t1' t2 t3)
   := by
   intro fh h2
   induction h2
@@ -215,40 +138,157 @@ namespace Star
   -- intro t1 _t2 t1' h; apply fh h
   -- exact h
 
-  variable [ReductionCompletion T R] [ReductionTriangle T R]
+  section
+    variable [SubstitutionType T] [SubstitutionTypeLaws T] [ReductionRespectsSubstitution T R]
 
-  theorem strip : R s t1 -> @Star T R s t2 -> ∃ t, @Star T R t1 t ∧ R t2 t := by
-  intro h1 h2
-  induction h2 generalizing t1
-  case _ t' => exists t1; apply And.intro; apply Star.refl; apply h1
-  case _ n' x y z _r1 r2 ih =>
-    replace ih := ih h1
-    cases ih
-    case _ w ih =>
-      replace r2 := ReductionTriangle.triangle r2
-      have lem := ReductionTriangle.triangle ih.2
-      replace lem := Star.step ih.1 lem
-      exists (ReductionCompletion.compl R y)
+    theorem subst_same σ : Star R t s -> Star R ([σ]t) ([σ]s) := by
+    intro h; induction h
+    case _ => apply Star.refl
+    case _ y z r1 r2 ih =>
+      replace r2 := ReductionRespectsSubstitution.subst σ r2
+      apply Star.step ih r2
+  end
 
-  theorem confluence : @Star T R s t1 -> @Star T R s t2 -> @Conv T R t1 t2 := by
-  intro h1 h2
-  induction h1 generalizing t2
-  case _ z =>
-    exists t2; apply And.intro
-    apply h2; apply Star.refl
-  case _ g3 s y t1 _r1 r2 ih =>
-    replace ih := ih h2
-    cases ih; case _ w ih =>
-      have lem := strip r2 ih.1
-      cases lem; case _ q lem =>
-        exists q; apply And.intro
-        apply lem.1; apply Star.step ih.2 lem.2
+  section
+    variable [SubstitutionType T] [SubstitutionTypeLaws T] [ReductionRespectsReducingSubstitution T R]
+
+    theorem subst σ τ :
+      (∀ n t, σ n = .su t -> ∃ t', τ n = .su t' ∧ R t t') ->
+      (∀ n k, σ n = .re k -> τ n = .re k) ->
+      Star R t s ->
+      Star R ([σ]t) ([τ]s)
+    := by
+    intro h1 h2 r; induction r
+    case _ => sorry
+    case _ y z r1 r2 ih =>
+      apply Star.step ih
+      apply ReductionRespectsReducingSubstitution.subst τ τ _ _ r2
+      case _ =>
+        intro n t h
+        sorry
+      case _ => sorry
+  end
+
+  section
+    variable [ReductionTriangle T R]
+
+    theorem strip : R s t1 -> Star R s t2 -> ∃ t, Star R t1 t ∧ R t2 t := by
+    intro h1 h2
+    induction h2 generalizing t1
+    case _ t' => exists t1; apply And.intro; apply Star.refl; apply h1
+    case _ x y z _r1 r2 ih =>
+      replace ih := ih h1
+      cases ih
+      case _ w ih =>
+        replace r2 := ReductionTriangle.triangle r2
+        have lem := ReductionTriangle.triangle ih.2
+        replace lem := Star.step ih.1 lem
+        exists (ReductionTriangle.compl R y)
+
+    theorem confluence : Star R s t1 -> Star R s t2 -> Conv R t1 t2 := by
+    intro h1 h2
+    induction h1 generalizing t2
+    case _ z =>
+      exists t2; apply And.intro
+      apply h2; apply Star.refl
+    case _ s y t1 _r1 r2 ih =>
+      replace ih := ih h2
+      cases ih; case _ w ih =>
+        have lem := strip r2 ih.1
+        cases lem; case _ q lem =>
+          exists q; apply And.intro
+          apply lem.1; apply Star.step ih.2 lem.2
+  end
 end Star
 
-namespace StarB
-  variable [ReductionCompletion T R] [ReductionTriangle T R]
+namespace Plus
+  theorem destruct : Plus R x z -> ∃ y, R x y ∧ Star R y z := by
+  intro r; induction r
+  case _ b r =>
+    exists b; apply And.intro r Star.refl
+  case _ r1 r2 ih =>
+    cases ih; case _ u ih =>
+      exists u; apply And.intro ih.1
+      apply Star.step ih.2 r2
 
-  theorem strip : R s t1 -> @StarB T R n s t2 -> ∃ t, @StarB T R n t1 t ∧ R t2 t := by
+  theorem stepr : R x y -> Plus R y z -> Plus R x z := by
+  intro r1 r2
+  induction r2 generalizing x
+  case _ r2 => apply Plus.step (Plus.start r1) r2
+  case _ r3 r4 ih => apply Plus.step (ih r1) r4
+
+  theorem stepr_from_star : R x y -> Star R y z -> Plus R x z := by
+  intro r1 r2
+  induction r2 generalizing x
+  case _ => apply Plus.start; apply r1
+  case _ r3 r4 ih => apply Plus.step (ih r1) r4
+end Plus
+
+namespace StarB
+  @[simp]
+  def star (f : T -> T) : Nat -> T -> T
+  | 0, t => t
+  | n + 1, t => star f n (f t)
+
+  theorem weaken k : StarB R g x y -> StarB R (g + k) x y := by
+  intro r; induction r generalizing k
+  case _ => constructor
+  case _ n _ _ _ _ r2 ih =>
+    have lem : n + 1 + k = n + k + 1 := by omega
+    rw [lem]; apply StarB.step (ih k) r2
+
+  theorem trans : StarB R g1 x y -> StarB R g2 y z -> StarB R (g1 + g2) x z := by
+  intro r1 r2; induction r2 generalizing g1 x
+  case _ n t => apply weaken n r1
+  case _ n a b c _ r2 ih => apply StarB.step (ih r1) r2
+
+  theorem promote (Rprm : ∀ {x y}, R1 x y -> R2 x y) :
+    StarB R1 n x y -> StarB R2 n x y
+  := by
+  intro r; induction r
+  case _ => constructor
+  case _ _ r ih => constructor; apply ih; apply Rprm r
+
+  theorem star_sound n t : (∀ t, R t (f t)) -> StarB R n t (star f n t) := by
+  intro h
+  have lem : ∀ {t n}, R (star f n t) (star f n (f t)) := by
+    intro t n; induction n generalizing t; simp; apply h _
+    case _ n ih => simp; apply ih
+  induction n
+  case _ => simp; constructor
+  case _ n ih =>
+    constructor; apply ih; simp; apply lem
+end StarB
+
+namespace ConvB
+  @[simp]
+  def convb [BEq T] (f : T -> T) (g1 g2 : Nat) (a b : T) : Bool :=
+    StarB.star f g1 a == StarB.star f g2 b
+
+  theorem weaken k1 k2 : ConvB R g1 g2 x y -> ConvB R (g1 + k1) (g2 + k2) x y := by
+  intro h; cases h; case _ w h =>
+    exists w; apply And.intro
+    apply StarB.weaken k1 h.1; apply StarB.weaken k2 h.2
+
+  theorem promote (Rprm : ∀ {x y}, R1 x y -> R2 x y) :
+    ConvB R1 g1 g2 x y -> ConvB R2 g1 g2 x y
+  := by
+  intro h; cases h; case _ w h =>
+    exists w; apply And.intro
+    apply StarB.promote Rprm h.1; apply StarB.promote Rprm h.2
+
+  theorem conv_sound [BEq T] [LawfulBEq T] : (∀ t, R t (f t)) -> convb f g1 g2 a b -> ConvB R g1 g2 a b := by
+  intro h1 h2; simp at h2
+  have lem1 := StarB.star_sound g1 a h1
+  have lem2 := StarB.star_sound g2 b h1
+  exists (StarB.star f g1 a); apply And.intro
+  apply lem1; rw [h2]; apply lem2
+end ConvB
+
+namespace StarB
+  variable [ReductionTriangle T R]
+
+  theorem strip : R s t1 -> StarB R n s t2 -> ∃ t, StarB R n t1 t ∧ R t2 t := by
   intro h1 h2
   induction h2 generalizing t1
   case _ t' => exists t1; apply And.intro; apply StarB.refl; apply h1
@@ -259,9 +299,9 @@ namespace StarB
       replace r2 := ReductionTriangle.triangle r2
       have lem := ReductionTriangle.triangle ih.2
       replace lem := StarB.step ih.1 lem
-      exists (ReductionCompletion.compl R y)
+      exists (ReductionTriangle.compl R y)
 
-  theorem confluence : @StarB T R g1 s t1 -> @StarB T R g2 s t2 -> @ConvB T R g2 g1 t1 t2 := by
+  theorem confluence : StarB R g1 s t1 -> StarB R g2 s t2 -> ConvB R g2 g1 t1 t2 := by
   intro h1 h2
   induction h1 generalizing t2
   case _ z =>
@@ -277,15 +317,15 @@ namespace StarB
 end StarB
 
 namespace Conv
-  theorem refl : @Conv T R t t := by
+  theorem refl : Conv R t t := by
   exists t; apply And.intro; apply Star.refl; apply Star.refl
 
-  theorem sym : @Conv T R x y -> @Conv T R y x := by
+  theorem sym : Conv R x y -> Conv R y x := by
   intro h; cases h; case _ w h =>
     exists w; apply And.intro; apply h.2; apply h.1
 
-  theorem trans [ReductionCompletion T R] [ReductionTriangle T R] :
-    @Conv T R x y -> @Conv T R y z -> @Conv T R  x z
+  theorem trans [ReductionTriangle T R] :
+    Conv R x y -> Conv R y z -> Conv R x z
   := by
   intro h1 h2
   cases h1; case _ w1 h1 =>
@@ -298,15 +338,15 @@ namespace Conv
 end Conv
 
 namespace ConvB
-  theorem refl : @ConvB T R g1 g2 t t := by
+  theorem refl : ConvB R g1 g2 t t := by
   exists t; apply And.intro; apply StarB.refl; apply StarB.refl
 
-  theorem sym : @ConvB T R g1 g2 x y -> @ConvB T R g2 g1 y x := by
+  theorem sym : ConvB R g1 g2 x y -> ConvB R g2 g1 y x := by
   intro h; cases h; case _ w h =>
     exists w; apply And.intro; apply h.2; apply h.1
 
-  theorem trans [ReductionCompletion T R] [ReductionTriangle T R] :
-    @ConvB T R gx gy1 x y -> @ConvB T R gy2 gz y z -> @ConvB T R (gx + gy2) (gz + gy1) x z
+  theorem trans [ReductionTriangle T R] :
+    ConvB R gx gy1 x y -> ConvB R gy2 gz y z -> ConvB R (gx + gy2) (gz + gy1) x z
   := by
   intro h1 h2
   cases h1; case _ w1 h1 =>
@@ -320,7 +360,7 @@ end ConvB
 
 def Reducible (t : T) := ∃ t', R t t'
 def Normal (t : T) := ¬ (@Reducible T R t)
-abbrev NormalForm (t : T) (t' : T) := @Star T R t t' ∧ @Normal T R t'
+abbrev NormalForm (t : T) (t' : T) := Star R t t' ∧ @Normal T R t'
 def WN (t : T) := ∃ t', @NormalForm T R t t'
 
 inductive SN (R : T -> T -> Prop) : T -> Prop where
@@ -353,13 +393,13 @@ induction h
 case _ z h1 _h2 =>
   apply h1 _ red
 
-theorem sn_preservation : SN R t -> @Star T R t t' -> SN R t' := by
+theorem sn_preservation : SN R t -> Star R t t' -> SN R t' := by
 intro h red
 induction red
 case _ => simp [*]
 case _ _ r2 ih => apply sn_preservation_step ih r2
 
-theorem sn_star : (∀ y, @Star T R t y -> SN R y) -> SN R t := by
+theorem sn_star : (∀ y, Star R t y -> SN R y) -> SN R t := by
 intro h
 constructor
 intro y r
@@ -369,7 +409,7 @@ theorem snplus_preservation_step : SNPlus R t -> R t t' -> SNPlus R t' := by
 intro h r; induction h; case _ z h _ =>
   apply h _ (Plus.start r)
 
-theorem snplus_preservation : SNPlus R t -> @Star T R t t' -> SNPlus R t' := by
+theorem snplus_preservation : SNPlus R t -> Star R t t' -> SNPlus R t' := by
 intro h r; induction r
 case _ => apply h
 case _ _ r2 ih =>
